\XeTeXinputencoding "GB2312"

\documentclass{beamer}
\usetheme{CambridgeUS}
\usepackage{xeCJK}
\setCJKmainfont{SimSun}
\usepackage{color,xcolor}            % 支持彩色文本、底色、文本框等
\usepackage{cite}                    % 支持引用
\usepackage{fontspec}
\usepackage{latexsym}
\usepackage{amsmath}                 % AMS LaTeX宏包
\usepackage{amssymb}                 % 用来排版漂亮的数学公式
\usepackage{amsbsy}
\usepackage{amsthm}
\usepackage{amsfonts}
\usepackage{mathrsfs}                % 英文花体字体
\usepackage{bm}                      % 数学公式中的黑斜体
\usepackage{relsize}                 % 调整公式字体大小?
\usepackage{pgfplots}
%\pagestyle{fancy}                    % 页眉页脚风格
\usetikzlibrary{shapes.geometric, arrows,matrix,positioning,calc}
%\setsansfont{楷体} % font name is case-sensitive
 \usepackage[%paperwidth=18.4cm, paperheight= 26cm,
            body={14.6true cm,22true cm},
            twosideshift=0 pt,
            %headheight=1.0true cm
            ]{geometry}

\usepackage[colorlinks,
            linkcolor=red,
            anchorcolor=blue,
            citecolor=green
            ]{hyperref}

\begin{document}
\title{ADER构造过程}
\frame{\titlepage}

\begin{frame}{ADER基本思想}
对于黎曼问题：
\begin{equation}
  \begin{aligned}
  &\partial_t U +\partial_x F(U) = 0 \\
 & U(x,0)=\left\{ \begin{array}{l}
	  U_L(x), x<x_{i+1/2}\\
	  U_R(x), x>x_{i+1/2}\\
  \end{array}\right.
\end{aligned}
\end{equation}

根据泰勒展开，在拉格朗日体系下，可以得到$\tau$时刻近似为
\begin{equation}
  U(x_{i+1/2},\tau)= U(x_{i+1/2},0+) +\sum_{k=1}^{r-1} \left[\frac{d ^k}{d t^k}U(x,t)(x_{i+1/2}, 0+) \right] \frac{\tau^k}{k!}
\end{equation}
其中$U(x_{i+1/2},0+)$是通过$U_L(x_{i+1/2})$和$U_L(x_{i-1/2})$构造的黎曼解求得的Godunov状态。
式中全导数可以通过如下形式得到，
\begin{equation}
  \frac{d}{dt} = \frac{\partial}{\partial t} + u\frac{\partial }{\partial x}
\end{equation}

\end{frame}
\begin{frame}{高阶全导数}
  \tiny
因此可以给出一到二阶高阶全导数形式如下
\begin{equation}
  \frac{dU}{dt} = \frac{\partial U}{\partial t} +u\frac{\partial U}{\partial x}
\end{equation}

\begin{equation}
  \begin{aligned}
  \frac{d^2U}{dt^2}& = \frac{d}{dt}( \frac{\partial U}{\partial t} +u\frac{\partial U}{\partial x})\\
  & =  \frac{\partial^2 U} {\partial t^2} +\frac{\partial u}{\partial t} \frac{\partial U}{\partial x} +2 u \frac{\partial ^2U}{\partial x \partial t} + u\frac{\partial u} {\partial x} \frac{\partial U} {\partial x} + u^2 \frac{\partial ^2 U} {\partial x^2}
\end{aligned}
\end{equation}

%\begin{equation}
%  \begin{aligned}
%  \frac{d^3U}{dt^3}& = \frac{d}{dt}( \frac{\partial^2 U} {\partial t^2} +\frac{\partial u}{\partial t} \frac{\partial U}{\partial x} +2 u \frac{\partial ^2U}{\partial x \partial t} + u\frac{\partial u} {\partial x} \frac{\partial U} {\partial x} + u^2 \frac{\partial ^2 U} {\partial x^2})\\
%  &= \frac{\partial^3 U} {\partial t^3} +\frac{}{}
%\end{aligned}
%\end{equation}
%
\end{frame}
\begin{frame}{高阶时间导数}
高阶时间导数求法：
\begin{equation}
  \begin{aligned}
&	\frac{\partial_U}{\partial t} = -A \frac{\partial U}{\partial x}  \\
& \frac{\partial ^2 U}{\partial x \partial t} = -\frac{\partial A}{\partial x}\frac{\partial U}{\partial x} -A \frac{\partial^2U}{\partial x^2}\\
&	\frac{\partial^2 U}{\partial t^2} = -\frac{\partial A}{\partial t}\frac{\partial U}{\partial x} -A \frac{\partial^2U}{\partial x \partial t}\\
&	\frac{\partial^3 U}{\partial x^2 \partial t} = -\frac{\partial^2 A}{\partial x^2}\frac{\partial U}{\partial x} -2\frac{\partial A }{\partial x} \frac{\partial^2U}{\partial x^2}-A\frac{\partial U^3}{\partial x^3}\\
&	\frac{\partial^3 U}{\partial x \partial t^2} = -\frac{\partial^2 A}{\partial x \partial t}\frac{\partial U}{\partial x} -\frac{\partial A }{\partial x} \frac{\partial^2U}{\partial x \partial t}- \frac{\partia A}{\partial t}\frac{\partial U^2}{\partial x^2} - A\frac{\partial ^3 U}{\partial x^2 \partial t}\\ 
&	\frac{\partial^3 U}{\partial t^3} = -\frac{\partial^2 A}{\partial t^2}\frac{\partial U}{\partial x}-\frac{\partial A }{\partial t} \frac{\partial^2U}{\partial x \partial t}- \frac{\partia A}{\partial t}\frac{\partial U^2}{\partial x \partial t} - A\frac{\partial ^3 U}{\partial x \partial t^2}\\ 
\end{aligned}
\end{equation}

\end{frame}

\begin{frame}{高阶空间导数和广义黎曼解}
  通过广义黎曼解，界面上空间导数发展方程为
  \begin{equation}
	\begin{aligned}
	\frac{\partial U_x^{(k)}}{\partial \tau} + A (U(x_{i+1/2}(0+), 0+)) \frac{\partial U_x^{(k)}}{\partial x} = 0 \\
	U_x^{(k)}(x_{i+1/2},0) =\left\{ \begin{aligned}
		P_L^{(k)}(x_{i+1/2}), \hspace{0.2cm} \text{if}  \hspace{0.2cm} x<x_{i+1/2},\\
		P_R^{(k)}(x_{i+1/2}), \hspace{0.2cm} \text{if}  \hspace{0.2cm} x>x_{i+1/2},\\
	\end{aligned} \right.
	\end{aligned}
  \end{equation}
  其中$A$为Jacob矩阵，$A=\frac{\partial F}{\partial U}$, $P_{L(R)}^{(k)} = \frac{\partial ^k U_{L(R)}(x)}{\partial x^k}$ 通过广义黎曼求解器可以得到更高阶空间导数。

  这里$A (U(x_{i+1/2}(0+), 0+))$ 为冻结矩阵，则可以通过如HLL构造
\begin{equation}
  U^{(k)}(x_{i+1/2},0) = \frac{s_R U^{(k)}_R-s_L U^{(k)}_L +AU^{(k)}_L-AU^{(k)}_R}{s_R-s_L}
\end{equation}
其中$s_L(R)$通过$U_L$和$U_R$构造。

\end{frame}

\begin{frame}{有限体积离散}
  在拉氏框架下，网格点随时间运动方程为
  \begin{equation}\label{eq:v}
	\frac{dx(t)}{dt} = u(x,t)
\end{equation}
对黎曼问题
 \begin{equation}\label{eq:1d}
   \left\{ \begin{aligned}
	   &\frac{\partial U}{\partial t} + \frac{\partial F}{\partial x} =0\\
	   &\partial _t s_{xx}+u\partial_xs_{xx}-\frac{4}{3}\partial_x u=0\\
	   &Q(x,t=0) = \left\{ \begin{aligned} 
		   Q_L, \hspace{0.2cm} \text{if} \hspace{0.2cm} x<0\\
		   Q_R, \hspace{0.2cm} \text{if} \hspace{0.2cm} x>0\\
	   \end{aligned} \right.
	 %  & \partial _t \rho +\partial_x(\rho u)=0\\
	 %  & \partial _t (\rho u)+\partial_x(\rho u^2 + p -s_{xx})=0\\
	 %  &\partial _t (\rho E)+\partial_x([\rho E + p -s_{xx}]u)=0\\
	 \end{aligned}
  \right.
\end{equation}
其中$U=(\rho,\rho u ,\rho E)$，$F = (\rho u, \rho u^2+p -s_{xx},(\rho E + p -s_{xx})u )$, $Q = (\rho,\rho u, \rho E)$。

\end{frame}

\begin{frame}{有限体积离散}

\end{frame}


\begin{frame}{三阶WENO格式下二阶空间导数构造方法}
\tiny
  We take the $U^{(1)}_L$ as an example, the same to $U_L$, we use two stencils $S(i-1,i)= c_{11} U_{i-1}+c_{12} U_{i}$ and $S(i,i+1) = c_{21}U_{i}+c_{22}U_{i+1}$ to construct the $U^{(1)L}_{i+1/2}$, 

  In an uniform mesh, the coefficients $c_{11}$ and $c_{12}$ are constructed as 
  \begin{equation}
	\frac{c_{11} U_{i-1} +c_{12} U_i-(c_{11} U_{i-2}+c_{12} U_{i-1})}{\Delta x^2} = \frac{\partial^2 U_i}{\partial x^2} +O(\Delta x)
  \end{equation}
  We get $c_{11}=-1$ and $c_{12}=1$, in a similar process, we can get $c_{21} =-1$ and $c_{22}=1$, so 

\begin{equation}
  \begin{aligned}
	q_1 = U_{i-1} -U_{i}\\ 
	q_2 = U_{i} -U_{i+1}\\ 
\end{aligned}
\end{equation}

Using $S(i-1,i,i+1)$ we can construct a 2nd order  approximation of $U^{(1)}_L$ 

\begin{equation}
  U^{(1)L}_{i+1/2} = \omega_1 q_1 +\omega_2 q_2
 \end{equation}

 where $\omega_i = \frac{\alpha _k}{\alpha_1+\alpha_2}$ and $\alpha_k = \frac{d_k}{(\beta_k+\varepsilon)^p}$, $d_k$ is the linear weights of $q_1$ and $q_2$ can be solved as 

 \begin{equation}
   \frac{d_1 q_1 + d_2 q_2}{\Delta x^2} = \frac{\partial^2 U_i}{\partial x^2} +O(\Delta x^2)
\end{equation}
Then we get $d_1 = \frac{1}{4}$ and $d_2 = \frac{3}{4}$. And the smoothness indicatros are 
\begin{equation}
  \beta_1 =q_1^2, \beta_2=q_2^2
\end{equation}



\end{frame}






\end{frame}

\begin{frame}{守恒方程有限体积离散}
\tiny
  在区域$(x_{i-1/2}^n,t^n) \rightarrow (x_{i+1/2}^n,t^n) \rightarrow  (x_{i+1/2}^n,t^{n+1}) \rightarrow   (x_{i+1/2}^{n+1},t^{n+1})$积分

\begin{equation}
  {\int \int}_{\omega} (\frac{\partial U}{\partial t} +\frac{\partial F}{\partial x})dx dt = 0 
\end{equation}
基于格林公式可以写作

\begin{equation}
  \oint_{\partial \omega}(Udx - F dt) = 0
\end{equation}
展开有
\begin{equation}
  \int_{x_{i-1/2}^{n+1}}^{x_{i+1/2}^{n+1}}Udx -\int_{x_{i-1/2}^{n}}^{x_{i+1/2}^{n}}Udx +\int_{x_{i-1/2}^{n+1}}^{x_{i-1/2}^{n}}Udx -\int_{x_{i+1/2}^{n+1}}^{x_{i+1/2}^{n}}Udx- \left(\int_{t^n} ^{t^{n+1}}F(x_{i-1/2},t)dt - \int_{t^n} ^{t^{n+1}}F(x_{i+1/2},t)dt\right) = 0
\end{equation}

将 Eq.(\ref{eq:v})带入有，
\begin{equation}
  \int_{x_{i-1/2}^{n+1}}^{x_{i+1/2}^{n+1}}Udx -\int_{x_{i-1/2}^{n}}^{x_{i+1/2}^{n}}Udx - \left[ \begin{aligned}  &\int_{t^n} ^{t^{n+1}}F(x_{i-1/2},t)-u(x_{i-1/2},t)Udt\\
							-&\int_{t^n} ^{t^{n+1}}F(x_{i+1/2},t)-u(x_{i+1/2},t)Udt\\
						\end{aligned} \right]
	= 0
  \end{equation}
  定义
  \begin{equation}
	f= F- uU
  \end{equation}
有
\begin{equation}\label{eq:con}
	  \int_{x_{i-1/2}^{n+1}}^{x_{i+1/2}^{n+1}}Udx -\int_{x_{i-1/2}^{n}}^{x_{i+1/2}^{n}}Udx - \left[ \int_{t^n} ^{t^{n+1}}f(x_{i-1/2},t)Udt
	  -\int_{t^n} ^{t^{n+1}}f(x_{i+1/2},t)Udt \right]
	= 0
  \end{equation}
\end{frame}
  \begin{frame}
  令单元平均值
  \begin{equation}
	\bar{U_i}^n= \frac{1}{\Delta x^n}  \int_{x_{i-1/2}^{n+1}}^{x_{i+1/2}^{n+1}}U(x,t^n)dx
  \end{equation}
  其中 $\Delta x^n = x_{i+1/2}^n - x_{i-1/2}^n$。
  因此Eq.(\ref{eq:con})变为
	
  \begin{equation}
	\bar{U_i}^{n+1} \Delta x_i^{n+1} - \bar{U_i}^n \Delta x_i^n - (F_{i-1/2}-F_{i+1/2}) = 0
  \end{equation}
  其中\begin{equation}
	F_{i+1/2} = \int_{t^n} ^{t^{n+1}}f(x_{i+1/2},t)dt
  \end{equation}

\end{frame}
\begin{frame}{Constitute equation}
  \tiny
  In the Lagrangian frame, the equation of the constitute model can be  written as 
  \begin{equation} \label{eq:constitute}
	\frac{\text{d}s_{xx}}{\text{d}t} = \frac{4\mu}{3} \frac{\partial u }{\partial x}
  \end{equation}
  For the cell-centered Lagrangian scheme, the geometrical conservation law is very important, that is, 
  \begin{equation}
	\frac{\dot{V}}{V} = \frac{\partial u}{\partial x}
  \end{equation}
  should be satisfied. In the one-dimensional case, the volume of the cell $I_i$ is evaluated by 
  \begin{equation} \label{eq:volume}
	V_i(t) = x_{i+1/2}(t) - x_{i-1/2}(t)
  \end{equation}
  Taking the material derivative on  the both sides of Eq.{\ref{eq:volume}}, we have 
  \begin{equation}
	\dot{V}_i(t) = u_{i+1/2}(t)- u _{i+1/2}(t)
  \end{equation}
We can get 
\begin{equation}
  \frac{\partial u}{\partial t}=\frac{\dot{V}_i(t)}{V_i} = \frac{u_{i+1/2}(t) - u_{i-1/2}(t)}{x_{i+1/2}-x_{i-1/2}}
\end{equation}
Then, The  semi-discrete formulation for Eq.{\ref{eq:constitute}} has the following form:
\begin{equation}
  \frac{ds_{xx}}{dt} = \frac{4\mu}{3}\frac{u_{i+1/2}- u_{i-1/2}}{\Delta x_i}
\end{equation}
%if we let
%\begin{equation}
%\Theta(i,\tau)=  \frac{4\mu}{3}u_{i+1/2}(\tau)
%
%- u_{i-1/2}(\tau)}{x_{i+1/2}(\tau) - x_{i-1/2}(\tau)}
%\end{equation}
%
%\begin{equation}
%  s_{xx}^{n+1} = s_{xx}^n+ \frac{}
%\sum_{k=1}^{n-1}\Theta(i,t_g)\omega_g \Delta t 
%\end{equation}

\end{frame}



  \begin{frame}{高斯积分}
	对于$F_{i+1/2}$采用高斯积分
	\begin{equation}
	F_{i+1/2} = \int_{t^n} ^{t^{n+1}}f(x_{i+1/2},t)dt =  \sum_{g=1} ^\alpha \omega_g f(U(x_{i+1/2(t_g)},t_g)) \Delta t 
  \end{equation}
其中 $\alpha$为高斯点个数， $\omega_g$为$g$点加权值。
\end{frame}


\begin{frame}{Gaussian quadrature}
  In numerical analysis, a quadrature rule is an approximation of the definite integral of a function, usually stated as a weighted sum of function values at specified points within the domain of integration. An n-point Gaussian quadrature rule named after Carl Friedrich Gauss, is a quadrature rule constructed to yield an exact result for polynomials of degree $2n-1$ or less by a suitable choice of the nodes $x_i$ and weightes $w_i$ for $i=1,\codts, n $. The most common domain of integration for such a rule is taken as $[-1,1]$, so the rule is stated as 
\begin{equation}
  \int_{-1}^1 f(x)dx \approx \sum_{i=0}^n \omega_i f(x_i)
\end{equation}
which is exact for polynomials of degree $2n-1$ or less. This exact rule is known as the Gauss-Legendre quadrature rule.


%其中含有$2n+2$个待定系数，$x_k$，$A_k(k=0,1,\cdots,n)$，当$x_k$为等距离节点时得到插值求积公式代数精度为$n$

\end{frame}
\begin{frame}{Guass-Legendre quadrature}
  \tiny
  For the simplest integration problem stated above, i.e., $f(x)$ is well-approximated by polynomials on $[-1,1]$, the associated orthogonal polynomials are Legrendre-polynomials, denoted by $P_n(x)$. The i-th Gauss node, $x_i$ is the i-th root of $P_n$ and the weights are given by the formula(Abramowitz & Stegun 1972, p.887) 
  \begin{equation}
	\omega_i = \frac{2}{(1-x_i^2)[P_n'(x_i)]^2}
\end{equation}

Some lower-order quadrature rules are tabulated below 
\begin{table}[htbp]
  \small 
  \centering
  \setlength{\belowcaptionskip}{10pt}
  \begin{tabular}{mmm}
	\toprule
	Number of points, $n$  & Points, $x_i$, & Weights, $\omega_i$ \\
	\midrule
	1 & 0 & 2 \\ 
	2 & $\pm \frac{1}{\sqrt{3}}$ & 1 \\ 
	3 & 0 ($\pm \sqrt{\frac{3}{5}}$) & $\frac{8}{9}$ ( $\frac{5}{9}$) \\   
	4 & $\pm \sqrt{\frac{3}{7}-\frac{2}{7}\sqrt{\frac{6}{5}}}$ ( $\pm \sqrt{\frac{3}{7}+\frac{2}{7}\sqrt{\frac{6}{5}}}$)& $\frac{18-\sqrt{30}}{36}$ (  $ \frac{18+\sqrt{30}}{36}$ ) \\
	\bottomrule
\end{tabular}
\end{table}

Change of interval

An integral over $[a,b]$ must be changed into an integral over $[-1,1]$ before applying the Gaussian quadrature rule. This change of interval can be done in the fllowing way
\begin{equation}
  \int_a^b f(x)dx = \frac{b-a}{2}\int_{-1}^1 f(\frac{b-a}{2}x+\frac{a+b}{2})dx
\end{equation}

对于区域$[0,\tau]$

\end{frame}

\begin{frame}{求解流程}
  \tiny
  \begin{equation}
	\begin{aligned}
	  & x_{i+1/2}^{n+1} = x_{i+1/2}^n+\sum_{g=1}^2 u(x_{i+1/2},t_g)\omega_g \Delta t\\
	  & \Delta x_i^{n+1} = x_{i+1/2}^{n+1} -x_{i-1/2}^{n+1}\\
	  & \Delta x_i^{n+1} \overline{U}_i^{n+1} = \Delta x_i^{n} \overline{U}_i^n + F_{i+1/2}-F_{i-1/2}\\
	  & \overline{\hat{s}_{xx}}_i^{n+1} = \overline{s_{xx}}_i^n + \frac{ \Theta_{i+1/2}- \Theta_{i-1/2}}{\Delta x^n}\\
	  & \overline{s_{xx}}_i^{n+1} = \Gamma( \overline{\hat{s}_{xx}}_i^{n+1})
	\end{aligned}
  \end{equation}
  其中
  \begin{equation}
	\begin{aligned}
	  &F_{i+1/2} = \sum_{g=1}^2 f(U(x_{i+1/2}), t_g) \omega_g \Delta t\\
	  &\Theta_{i+1/2} = \sum_{g=1}^2 \frac{4}{3}\mu u(x_{i+1/2},t_g) \omega_g \Delta t\\
	\end{aligned}
  \end{equation}

  通过泰勒展开
  \begin{equation}
	  U(x_{i+1/2},\tau) = U(x_{i+1/2},0) + \sum_{k=1}^{n-1} \frac{d^kU}{dt^k}\frac{\tau^n}{n!}
	\end{equation}
  \end{frame}
  \begin{frame}{求解流程}
	\tiny
其中全导数

\begin{equation}
  \begin{aligned}
  &\frac{dU}{dt} = \frac{\partial U}{\partial t} +u\frac{\partial U}{\partial x}\\
  &\frac{d^2U}{dt^2} = \frac{d}{dt}( \frac{\partial U}{\partial t} +u\frac{\partial U}{\partial x})\\
  & =  \frac{\partial^2 U} {\partial t^2} +\frac{\partial u}{\partial t} \frac{\partial U}{\partial x} +2 u \frac{\partial ^2U}{\partial x \partial t} + u\frac{\partial u} {\partial x} \frac{\partial U} {\partial x} + u^2 \frac{\partial ^2 U} {\partial x^2}
\end{aligned}
\end{equation}
时间导数又可以转化为空间导数
\begin{equation}
  \begin{aligned}
&	\frac{\partial U}{\partial t} = -A \frac{\partial U}{\partial x}  \\
& \frac{\partial ^2 U}{\partial x \partial t} = -\frac{\partial A}{\partial x}\frac{\partial U}{\partial x} -A \frac{\partial^2U}{\partial x^2}\\
&	\frac{\partial^2 U}{\partial t^2} = -\frac{\partial A}{\partial t}\frac{\partial U}{\partial x} -A \frac{\partial^2U}{\partial x \partial t}\\
\end{aligned}
\end{equation}
最终需要构造高阶空间导数。
根据重构 如WENO3可以构造二阶精度的$U_L(x_{i+1/2},0)$和$U_R(x_{i+1/2},0)$同样可以构造一阶精度的$U^{(1}_L(x_{i+1/2},0)$和$U^{(1)}_R(x_{i+1/2},0)$。WENO5可以构造四阶的$U_{L(R)}(x_{i+1/2},0)$ $\dots$ 一阶精度的
$U^{(3)}_{L(R)}(x_{i+1/2},0)$。

通过黎曼求解器可以根据$U_{L(R)}(x_{i+1/2},0)$求得$U(x_{i+1/2},0)$，同样的通过广义黎曼求解器可以根据$U^{(k)}_{L(R)}(x_{i+1/2},0)$得到$U^{(k)}(x_{1+1/2})$。

\end{frame}

\begin{frame}{$A$和$dA$}
  \tiny
  \begin{equation}
	A=\left(
	\begin{array}{llll}
	  0 & 1 & 0 & 0 \\
	  -u^2+\frac{\partial p }{\partial \rho} +\Gamma(\frac{u^2}{2}-e)& u(2-\Gamma)& \Gamma & -1\\
	  (\Gamma(\frac{u^2}{2}-e)-e+\frac{\sigma_x}{\rho}+\frac{\partial p }{\partial \rho})u &  -\Gamma u^2-\frac{\sigma_x}{\rho} +e & (1+\Gamma)u & -u \\
	  \frac{4}{3}\mu \frac{u}{\rho} &-\frac{4}{3}\mu \frac{1}{\rho}& 0 & u\\
	\end{array}
  \right)
\end{equation}
where,
$e=E-\frac{u^2}{2}$, $\Gamma = \frac{\Gamma_0 \rho_0}{\rho}$, $\sigma_x= -p+s_{xx}$, $\frac{\partial p}{\partial \rho} = a_0^2 f'(\eta)$  

\end{frame}

\begin{frame}
  \tiny
\begin{equation} 
 \begin{aligned}
  & dA(1,1) = 0
  \hspace{0.3cm}  dA(1,2) = 0
   \hspace{0.3cm}  dA(1,3) = 0
    \hspace{0.3cm} dA(1,4) = 0\\
  & dA(2,1) =-2udu + a_0^2 f''(\eta)\frac{d\rho}{\rho_0}+d\Gamma(\frac{u^2}{2}-e)+\Gamma(udu-de)\\
  & dA(2,2) = du(2-\Gamma)-ud\Gamma \\
  & dA(2,3)= d\Gamma \\ 
  & dA(2,4) = 0 \\
  & dA(3,1) = (\Gamma(\frac{u^2}{2}-e)-e+\frac{\sigma_x}{\rho}+\frac{\partial p }{\partial \rho})du + (d\Gamma(\frac{u^2}{2}-e)+\Gamma(udu-de) -de + \frac{d\sigma_x}{\rho} -\frac{\sigma_x d\rho}{\rho^2} +  a_0^2 f''(\eta)\frac{d\rho}{\rho_0})u\\
  &  dA(3,2) =- d\Gamma u^2-2u\Gamma -\frac{d\sigma_x}{\rho} +\frac{\sigma_x d\rho}{\rho^2} +de \\
  & dA(3,3)= (1+\Gamma)du+d\Gamma u \\
  & dA(3,4)=  -du \\  
  & dA(4,1) =   \frac{4}{3}\mu \frac{du}{\rho}- \frac{4}{3}\mu \frac{u d\rho}{\rho^2} \\
   & dA(4,2)=  \frac{4}{3}\mu \frac{d\rho}{\rho^2}  \\
   & dA(4,3) = 0\\ 
  & dA(4,4)= du \\
\end{aligned}
\end{equation}
where
$de=dE-udu$,$d\Gamma = -\frac{\Gamma_0 \rho_0 d\rho}{\rho^2}$, $d\sigma_x = -dp+ds_{xx}$.


\end{frame}

\begin{frame}{sub-cell WENO-3 construct}
  \tiny

  First, define sub-cell points
  The sub-cell points $x_i^{(k)}$, $k=1,\dots,2r-1$ in $I_i$ are given by 
  \begin{equation}
	x_i^{(k)} =x_{i-1/2} + \frac{k-1}{2r-3}\Delta x
  \end{equation}
  For third-order scheme there are is no need of sub-cell points, $x_i^{(1)} = x_{(i-1/2)}$,$x_i^{2}=x_{(i+1/2)}$.

  Step 2 Reconstruct (2r-2) point-wise values of $u$
  Using $p_{WENO}^{2r-1}$ to get $u_i^{(k)}$
  \begin{equation}
	p_{WENO}^{2r-1} = \sum_{k=0}^{r-1} \omega_k q_k^r(x, \bar{u}_{i-r+1+k},\cdots,\bar{u}_{i+k}) 
  \end{equation}

\begin{equation}
  u_i^{(k)}= u(x_i^{(k)}) + e_i^{(k)} (\Delta x)^{2r-1}
\end{equation}

Step 3, Construct $p_i(x)$
Ansatz $p_i(x)$ of $u$ in $I_i$ as follows
\begin{equation}
  p_i(x)=\sum_{l=0}^{2r-2} a_l(\frac{x-x_{i-1/2}}{\Delta x})^l
\end{equation}

By the equation 
\begin{equation}
  \left\{
  \begin{aligned}
&	p_i(x_i^{(l)}) = u_i^{(l)}, \hspace{0.2cm} l=0,\cdots,2r-2\\
&	\frac{1}{\Delta x} \int_{I_i}p_i(x) dx = \bar{u}_i 
  \end{aligned}
\right.
\end{equation}
\end{frame}

\begin{frame}
For the third-order WENO scheme
\begin{equation}
  \begin{aligned}
	U_i^{(1)} = U_{(i-1/2)}\\
	U_i^{(2)} = U_{(i+1/2)}\\
\end{aligned}
\end{equation}

\begin{equation}
  \begin{aligned}
	&a_0= U_i^{(1)}\\
	&a_1 = 6\bar{U} -2 U_i^{(2)}-4U_i^{(1)}\\
	&a_2=3(U_i^{(1)}+U_i^{(2)}-2\bar{U})
  \end{aligned}
\end{equation}



\end{frame}
\begin{frame}{$U^{(i)}_L$}
\tiny
For  each cell $I_j$, we have two stencils $S_j=(x_{j-\frac{3}{2}},x_{j-\frac{1}{2}}, x_{j+\frac{1}{2}})$ and $S_{j+1} = (x_{j-\frac{1}{2}}, x_{j+\frac{1}{2}}, x_{j+\frac{3}{2}})$ corresponding to $I_j = [x_{j-\frac{1}{2}}, x_{j+\frac{1}{2}}]$. On these two stencils, we obtain two interpolations 
  \begin{equation}
	p'_j(x) = \bat{u}_j+\frac{\bar{u}_j-\bar{u}_{j-1}}{h}(x-x_j),
	p'_{j+1}(x) = \bar{u}_j+\frac{\bar{u}_{j+1}-\bar{u}_{j}}{h}(x-x_j)
  \end{equation}
  with the smoothness indicators $IS_j=(\bar{u}_j-\bar{u}_{j-1})^2$ and $IS_{j+1} = (\bar{u}_{j+1}- \bar{u}_j)^2$ 
  Then we can get the left-hand reconstruction 
  \begin{equation}
	R_j(x) = \frac{\alpha_0}{\alpha_0+\alpha_1} p'_j(x) +  \frac{\alpha_1}{\alpha_0+\alpha_1} p'_{j+1}(x)
\end{equation}
where $\alpha_0 = C_0/(\varepsilon + IS_j)^2$, $\alpha_1= C_1/(\varepsilon + IS_{j+1})$,  
$C_0$ and $C_1$ are the optimal weight of $u$ at position $x$, given by solving 
\begin{equation}
  q^{3}(x,\bar{u}_{i-1},\bar{u}_{i},\bar{u}_{i+1}) = \sum_{k=0}^1 C_0q_0(x,\bar{u}_{i-1+k},\bar{u}_{i+k})
\end{equation}

For convenient to understand, here we set $\beta = (x-x_i)/\Delta x$, $C_0$ and $C_1$ are
\begin{equation}
  C_0=1-\frac{\beta_a}{\beta}
  C_1=\frac{\beta_a}{\beta}
\end{equation}
where $\beta_a= 3\beta^2+3\beta -\frac{1}{4}$.

The we can get the subcell approximation of $u$ in $I_j$ as 
\begin{equation}
  p_j(x)=\sum_{l=0}^{2}a_l (\frac{x-x_{j+1/2}}{\Delta x})^l
\end{equation}

\end{frame}
\begin{frame}
  \tiny
where 
\begin{equation}
  \begin{aligned}
	&a_0= U_i^{(1)}\\
	&a_1 = 6\bar{U} -2 U_i^{(2)}-4U_i^{(1)}\\
	&a_2=3(U_i^{(1)}+U_i^{(2)}-2\bar{U})
  \end{aligned}
\end{equation}
and $u_i^{(1)}=R_j(x_{i-1/2})$,$u_i^{(2)} = R_j(x_{i+1/2})$.

So 
\begin{equation}
  \begin{aligned}
  & \frac{\partial p_j}{\partial x}(x) = \frac{a_1}{\Delta x} +\frac{2a_2(x-x_{i-1/2})}{\Delta x^2} \\  
  & \frac{\partial^ 2 p_j}{\partial x^2}(x) = \frac{2a_2}{\Delta x^2} 
\end{aligned}
\end{equation}












 



\end{frame}

\begin{frame}{$U^{(i)}_R$}
\tiny
For  each cell $I_j$, we have two stencils $S_j=(x_{j-\frac{3}{2}},x_{j-\frac{1}{2}}, x_{j+\frac{1}{2}})$ and $S_{j+1} = (x_{j-\frac{1}{2}}, x_{j+\frac{1}{2}}, x_{j+\frac{3}{2}})$ corresponding to $I_j = [x_{j-\frac{1}{2}}, x_{j+\frac{1}{2}}]$. On these two stencils, we obtain two interpolations 
  \begin{equation}
	p'_j(x) = \bat{u}_j+\frac{\bar{u}_j-\bar{u}_{j-1}}{h}(x-x_j)
  \end{equation}
  and
  \begin{equation}
	p'_{j+1}(x) = \bar{u}_j+\frac{\bar{u}_{j+1}-\bar{u}_{j}}{h}(x-x_j)
  \end{equation}
  with the smoothness indicators $IS_j=(\bar{u}_j-\bar{u}_{j-1})^2$ and $IS_{j+1} = (\bar{u}_{j+1}- \bar{u}_j)^2$ 
  Then we can get the left-hand reconstruction 
  \begin{equation}
	u_L(x) = \frac{\alpha_0}{\alpha_0+\alpha_1} p'_j(x) +  \frac{\alpha_1}{\alpha_0+\alpha_1} p'_{j+1}(x)
\end{equation}
where $\alpha_0 = C_0/(\varepsilon + IS_j)^2$, $\alpha_1= C_1/(\varepsilon + IS_{j+1})$,  
$C_0$ and $C_1$ are the optimal weight of $u$ at position $x$, given by solving 
\begin{equation}
  q^{3}(x,\bar{u}_{i-1},\bar{u}_{i},\bar{u}_{i+1}) = \sum_{k=0}^1 C_0q_0(x,\bar{u}_{i-1+k},\bar{u}_{i+k})
\end{equation}

For convenient to understand, here we set $\beta = (x-x_i)/\Delta x$, $C_0$ and $C_1$ are
\begin{equation}
  C_0=1-\frac{\beta_a}{\beta}
  C_1=\frac{\beta_a}{\beta}
\end{equation}
where $\beta_a= 3\beta^2+3\beta -\frac{1}{4}$.

The we can get the subcell approximation of $u$ in $I_j$ as 
\begin{equation}
  p_j(x)=\sum_{l=0}^{2}a_l (\frac{x-x_{j+1/2}}{\Delta x})^l
\end{equation}

where 
\begin{equation}
  \begin{aligned}
	&a_0= U_i^{(1)}\\
	&a_1 = 6\bar{U} -2 U_i^{(2)}-4U_i^{(1)}\\
	&a_2=3(U_i^{(1)}+U_i^{(2)}-2\bar{U})
  \end{aligned}
\end{equation}
and $u_i^{(1)}=u_L(x_{i-1/2})$,$u_i^{(2)} = u_L(x_{i+1/2})$.

So 
\begin{equation}
  \begin{aligned}
  \frac{\partial^ 1 u_L}{\partial x}(x) = \frac{a_1}{\Delta x} +\frac{2a_2(x-x_{i-1/2})}{\Delta x^2} \\  
  \frac{\partial^ 2 u_L}{\partial x^2}(x) = \frac{2a_2}{\Delta x^2} 
\end{aligned}
\end{equation}












 



\end{frame}







		
\end{document}

